src/Amortization.v
@@ -6,6 +6,34 @@ Require Import Kami.ModularFacts Kami.RefinementFacts.
 Set Implicit Arguments.
 Set Asymmetric Patterns.
 
+(*** Move to SemFacts.v *)
+
+Lemma multistep_app:
+  forall m ll1 ll2 o n,
+    Multistep m o n (ll1 ++ ll2) ->
+    exists n', Multistep m o n' ll2 /\ Multistep m n' n ll1.
+Proof.
+  induction ll1; simpl; intros.
+  - eexists; split; eauto.
+    constructor; auto.
+  - inv H; specialize (IHll1 _ _ _ HMultistep); dest.
+    eexists; split; eauto.
+    constructor; auto.
+Qed.
+
+Lemma multistep_app_inv:
+  forall m ll1 ll2 o n n',
+    Multistep m o n' ll2 ->
+    Multistep m n' n ll1 ->
+    Multistep m o n (ll1 ++ ll2).
+Proof.
+  induction ll1; simpl; intros.
+  - inv H0; auto.
+  - inv H0; constructor; eauto.
+Qed.
+
+(*** End *)
+
 (** Extension of the restrict notion *)
 
 Definition restrictLabel (l: LabelT) (d: list string): LabelT :=
@@ -30,15 +58,11 @@ Inductive AmortizedSeq: LabelSeqT (* amortization *) -> LabelSeqT -> LabelSeqT -
     forall amt ll1 ll2,
       AmortizedSeq amt ll1 ll2 ->
       forall l1, AmortizedSeq (amt ++ [l1]) (l1 :: ll1) (emptyMethLabel :: ll2)
-| AmortizedCsm:
-    forall amt l2 ll1 ll2,
-      AmortizedSeq (l2 :: amt) ll1 ll2 ->
-      AmortizedSeq amt (emptyMethLabel :: ll1) (l2 :: ll2)
 | AmortizedBoth:
     forall amt l2 ll1 ll2,
       AmortizedSeq (l2 :: amt) ll1 ll2 ->
       forall l1, AmortizedSeq (amt ++ [l1]) (l1 :: ll1) (l2 :: ll2)
-| AmortizedNone:
+| AmortizedSame:
     forall ll1 ll2,
       AmortizedSeq nil ll1 ll2 ->
       forall l, AmortizedSeq nil (l :: ll1) (l :: ll2).
@@ -65,6 +89,16 @@ Section AboutCertainMethods.
           EquivalentLabelWithout l1 l2 ->
           EquivalentLabelSeqWithout (l1 :: ll1) (l2 :: ll2).
 
+  Lemma equivalentLabelSeqWithout_with:
+    forall ll1 ll2,
+      Forall (fun l => M.KeysSubset (defs l) fs) ll1 ->
+      Forall (fun l => M.KeysSubset (calls l) fs) ll1 ->
+      Forall (fun l => M.KeysSubset (defs l) fs) ll2 ->
+      Forall (fun l => M.KeysSubset (calls l) fs) ll2 ->
+      EquivalentLabelSeqWithout ll1 ll2.
+  Proof.
+  Admitted.
+
   Definition traceRefinesAmort m1 m2 :=
     forall s1 sig1,
       Behavior m1 s1 sig1 ->
@@ -73,11 +107,25 @@ Section AboutCertainMethods.
         EquivalentLabelSeqWithout sig1 sig2 /\
         exists amt, AmortizedSeq amt (restrictLabelSeq sig1 fs) (restrictLabelSeq sig2 fs).
 
+  Definition traceRefinesAmortA m1 m2 :=
+    forall s1 sig1,
+      Behavior m1 s1 sig1 ->
+      forall amt col2,
+        AmortizedSeq amt (restrictLabelSeq sig1 fs) col2 ->
+        exists s2 sig2,
+          Behavior m2 s2 sig2 /\
+          EquivalentLabelSeqWithout sig1 sig2 /\
+          col2 = restrictLabelSeq sig2 fs.
+
 End AboutCertainMethods.
 
 Notation "ma <<~[ p ]{ fs } mb" :=
   (traceRefinesAmort (liftToMap1 p) fs ma mb)
     (at level 100, format "ma  <<~[  p  ]{  fs  }  mb").
+
+Notation "ma <|~[ p ]{ fs } mb" :=
+  (traceRefinesAmortA (liftToMap1 p) fs ma mb)
+    (at level 100, format "ma  <|~[  p  ]{  fs  }  mb").
 
 Section TwoModuleFacts.
   Variables (m1 m2: Modules).
@@ -121,30 +169,167 @@ Section TwoModuleFacts.
   Qed.
 
 End TwoModuleFacts.
-  
+
+Section AmortARefl.
+  Variables (m: Modules)
+            (fs: list string).
+  Hypothesis (Hwf: ModEquiv type typeUT m)
+             (Habs: SubList (getExtMeths m) fs).
+
+  Lemma absorber_behavior_restrictLabelSeq:
+    forall n ll,
+      Multistep m (initRegs (getRegInits m)) n ll ->
+      restrictLabelSeq ll fs = ll.
+  Proof.
+    intros.
+    pose proof (multistep_defs_ext_in Hwf H).
+    pose proof (multistep_calls_ext_in Hwf H).
+    clear H.
+    induction ll; simpl; intros; auto.
+    inv H0; inv H1.
+    f_equal; auto.
+    destruct a as [a d c]; unfold restrictLabel; simpl in *.
+    f_equal; auto.
+    - apply M.restrict_KeysSubset; auto.
+      eapply M.KeysSubset_SubList; eauto.
+    - apply M.restrict_KeysSubset; auto.
+      eapply M.KeysSubset_SubList; eauto.
+  Qed.
+
+  Lemma absorber_amortizeSeq_invariant:
+    forall amt ll1 ll2,
+      AmortizedSeq amt ll1 ll2 ->
+      forall n1,
+        Multistep m (initRegs (getRegInits m)) n1 ll1 ->
+        forall n2,
+          Multistep m (initRegs (getRegInits m)) n2 ll2 ->
+          Multistep m (initRegs (getRegInits m)) n1 ((rev amt) ++ ll2).
+  Proof.
+    induction 1; simpl; intros; auto.
+    - rewrite rev_app_distr; simpl.
+      inv H0; inv H1.
+      specialize (IHAmortizedSeq _ HMultistep _ HMultistep0).
+      apply multistep_app in IHAmortizedSeq; dest.
+      constructor; auto.
+      apply multistep_app_inv with (n':= x).
+      + replace x with (M.union (M.empty _) x) by meq.
+        constructor; auto.
+        apply step_empty; auto.
+      + auto.
+    - inv H0; inv H1.
+      rewrite rev_app_distr; simpl.
+      constructor; auto.
+      replace (rev amt ++ l2 :: ll2) with (rev (l2 :: amt) ++ ll2)
+        by (simpl; rewrite <-app_assoc; simpl; reflexivity).
+      eapply IHAmortizedSeq; eauto.
+    - inv H0; inv H1.
+      constructor; eauto.
+  Qed.
+
+  Lemma traceRefinesAmortA_refl':
+    forall amt sig1 sig2,
+      AmortizedSeq amt sig1 sig2 ->
+      forall s1,
+        Multistep m (initRegs (getRegInits m)) s1 sig1 ->
+        exists s2, Behavior m s2 sig2.
+  Proof.
+    induction 1; simpl; intros.
+    - inv H; eexists; repeat constructor.
+    - inv H0; specialize (IHAmortizedSeq _ HMultistep).
+      destruct IHAmortizedSeq as [s2 ?].
+      eexists; repeat constructor.
+      + inv H0; eauto.
+      + apply step_empty; auto.
+    - inv H0; specialize (IHAmortizedSeq _ HMultistep); destruct IHAmortizedSeq as [s2 ?].
+      inv H0; pose proof (absorber_amortizeSeq_invariant H HMultistep HMultistepBeh).
+      simpl in H0.
+      rewrite <-app_assoc in H0; apply multistep_app in H0.
+      dest; simpl in *.
+      eexists; econstructor; eauto.
+    - inv H0; specialize (IHAmortizedSeq _ HMultistep); destruct IHAmortizedSeq as [s2 ?].
+      inv H0; pose proof (absorber_amortizeSeq_invariant H HMultistep HMultistepBeh).
+      simpl in H0.
+      eexists; repeat constructor; eauto.
+  Qed.
+
+  Lemma traceRefinesAmortA_refl:
+    traceRefinesAmortA id fs m m.
+  Proof.
+    unfold traceRefinesAmortA; intros.
+    erewrite absorber_behavior_restrictLabelSeq in H0; eauto; [|inv H; eauto].
+    inv H.
+    pose proof (traceRefinesAmortA_refl' H0 HMultistepBeh).
+    destruct H as [s2 ?].
+    exists s2; exists col2; split; auto.
+    split.
+    - inv H.
+      apply equivalentLabelSeqWithout_with.
+      + pose proof (multistep_defs_ext_in Hwf HMultistepBeh).
+        clear -Habs H; induction sig1; simpl; intros; auto.
+        inv H; constructor; auto.
+        eauto using M.KeysSubset_SubList.
+      + pose proof (multistep_calls_ext_in Hwf HMultistepBeh).
+        clear -Habs H; induction sig1; simpl; intros; auto.
+        inv H; constructor; auto.
+        eauto using M.KeysSubset_SubList.
+      + pose proof (multistep_defs_ext_in Hwf HMultistepBeh0).
+        clear -Habs H; induction col2; simpl; intros; auto.
+        inv H; constructor; auto.
+        eauto using M.KeysSubset_SubList.
+      + pose proof (multistep_calls_ext_in Hwf HMultistepBeh0).
+        clear -Habs H; induction col2; simpl; intros; auto.
+        inv H; constructor; auto.
+        eauto using M.KeysSubset_SubList.
+    - inv H; eapply eq_sym, absorber_behavior_restrictLabelSeq; eauto.
+  Qed.
+
+End AmortARefl.
+
+(** * This is an interacting case within amortized labels. *)
+(* NOTE1: we need one more interacting case within non-amortizing labels.
+ * Informally, the statement should be like:
+ * m1 <<~[p]{fs1} m2 -> m3 <<~[p]{fs2} m4 -> m1 ++ m3 <<~[id]{fs1 ++ fs2} m2 ++ m4.
+ *)
+(* NOTE2: we certainly also need a non-interacting case.
+ * Informally, the statement should be like:
+ * m1 <<~[p]{fs1} m2 -> m3 <<~[p]{fs2} m4 -> m1 ++ m3 <<~[p]{fs1 ++ fs2} m2 ++ m4.
+ *)
 Section Modularity.
-  Variables (m1 m2 ctxt: Modules).
+  Variables (m1 m2 m3 m4: Modules).
   Variable fs: list string.
   
   Hypotheses (Hwf1: ModEquiv type typeUT m1)
              (Hwf2: ModEquiv type typeUT m2)
-             (Hwfc: ModEquiv type typeUT ctxt)
+             (Hwf3: ModEquiv type typeUT m3)
+             (Hwf4: ModEquiv type typeUT m4).
+  (* (Hrdisj: DisjList (namesOf (getRegInits m1)) (namesOf (getRegInits m2))) *)
+  (* (Hddisj: DisjList (getDefs m1) (getDefs m2)) *)
+  (* (Hcdisj: DisjList (getCalls m1) (getCalls m2)) *)
+  (* (Hvr1: ValidRegsModules type m1) *)
+  (* (Hvr2: ValidRegsModules type m2) *)
 
-             (Hrdisj: DisjList (namesOf (getRegInits m1)) (namesOf (getRegInits m2)))
-             (Hddisj: DisjList (getDefs m1) (getDefs m2))
-             (Hcdisj: DisjList (getCalls m1) (getCalls m2))
-             (Hvr1: ValidRegsModules type m1)
-             (Hvr2: ValidRegsModules type m2)
-
-             (Hemc: getExtMeths ctxt = fs)
-             (Hvrc: ValidRegsModules type ctxt).
-
-  Theorem traceRefinesAmort_modular:
+  Theorem traceRefinesAmort_absorbed_modular:
     forall vp,
       traceRefinesAmort (liftToMap1 vp) fs m1 m2 ->
-      (m1 ++ ctxt)%kami <<=[vp] (m2 ++ ctxt)%kami.
+      traceRefinesAmortA (liftToMap1 vp) fs m3 m4 ->
+      (m1 ++ m3)%kami <<=[vp] (m2 ++ m4)%kami.
   Proof.
   Admitted.
 
 End Modularity.
+
+Corollary traceRefinesAmort_refl_modular:
+  forall m1 m2 fs,
+    ModEquiv type typeUT m1 ->
+    ModEquiv type typeUT m2 ->
+    traceRefinesAmort id fs m1 m2 ->
+    forall ctxt,
+      ModEquiv type typeUT ctxt ->
+      SubList (getExtMeths ctxt) fs ->
+      (m1 ++ ctxt)%kami <<== (m2 ++ ctxt)%kami.
+Proof.
+  intros.
+  eapply traceRefinesAmort_absorbed_modular; eauto; rewrite idElementwiseId; eauto.
+  apply traceRefinesAmortA_refl; auto.
+Qed.
 
